theories/Semantics/Temporal_Transition.v
@@ -19,9 +19,6 @@ Module SRE := SREnvironment.
 Module ST := Stock.
 Module RC := RContext.
 
-Section temporal.
-
-Hypothesis put : nat -> resource * (option Λ) -> Λ.
 
 
 (** *** Well-formed environments-context *)
@@ -61,8 +58,8 @@ Definition put_aux (r: resource) (V: 𝐕) :=
     | _ => None 
   end.
 
-Definition puts (n : nat) (R : 𝐄) (V: 𝐕) :=
-  SRE.foldkeys (fun k acc => ⌈k ⤆ put n (k,(put_aux k V))⌉ acc)%sr R ∅%sr.
+Definition puts (put : resource * (option Λ) -> Λ) (R : 𝐄) (V: 𝐕) :=
+  SRE.foldkeys (fun k acc => ⌈k ⤆ put (k,(put_aux k V))⌉ acc)%sr R ∅%sr.
 
 (** *** Initialize the input resource environment 
 
@@ -75,7 +72,7 @@ Definition init_input_env (R : 𝐄) (W : 𝐖) : 𝐕 :=
 
 (** *** Temporal transition *)
 
-Definition temporal (n : nat) (R R': 𝐄) (P P' : Λ) (W W' : 𝐖) :=
+Definition temporal (put : resource * (option Λ) -> Λ) (R R': 𝐄) (P P' : Λ) (W W' : 𝐖) :=
 
   (** (1) Initialize the local memory [Vin] with global and local resources. *)
   let Vin := init_input_env R W in
@@ -85,7 +82,7 @@ Definition temporal (n : nat) (R R': 𝐄) (P P' : Λ) (W W' : 𝐖) :=
   ⪡ Vin ; unit ; P ⪢ ⭆ ⪡ Vout ; _tv ; P' ; Wnew ⪢ /\
 
   (** (3) Update the global and local resources. *)               
-  (R' = puts n R Vout)%sr  /\
+  (R' = puts put R Vout)%sr  /\
   (W' = (ST.update_locals (([⧐ (W⁺)%sk – (Vout⁺ - (W⁺)%sk)%re] W) ++ Wnew) Vout))%sk.
 
 Notation "# n '⟦' R ';' W ';' P '⟧' '⟾' '⟦' S1 ';' W1 ';' P1 '⟧'" := (temporal n R S1 P P1 W W1) 
@@ -95,15 +92,19 @@ Notation "# n '⟦' R ';' W ';' P '⟧' '⟾' '⟦' S1 ';' W1 ';' P1 '⟧'" := (
 
 (** *** [puts] properties *)
 
-#[export] Instance aux_eq (n : nat) (V: 𝐕) : Proper (eq ==> SRE.eq ==> SRE.eq) 
-  (fun (k: resource) (acc : SRE.t) => (⌈k ⤆ put n (k, put_aux k V) ⌉ acc)%sr).
+Section put_props.
+
+Variable put : resource * (option Λ) -> Λ. 
+
+#[export] Instance aux_eq (V: 𝐕) : Proper (eq ==> SRE.eq ==> SRE.eq) 
+  (fun (k: resource) (acc : SRE.t) => (⌈k ⤆ put (k, put_aux k V) ⌉ acc)%sr).
 Proof.
   intros r' r Heqr R R' HeqR; subst.
   now rewrite HeqR.
 Qed.
 
-Lemma aux_diamond (n : nat) (V: 𝐕) : SRE.Diamond SRE.eq 
-  (fun (k: resource) (_: Λ) (acc : SRE.t) => (⌈ k ⤆ put n (k, put_aux k V) ⌉ acc)%sr).
+Lemma aux_diamond  (V: 𝐕) : SRE.Diamond SRE.eq 
+  (fun (k: resource) (_: Λ) (acc : SRE.t) => (⌈ k ⤆ put (k, put_aux k V) ⌉ acc)%sr).
 Proof.
   intros r r' _ _ R1 R R' Hneq Heq Heq'.
   rewrite <- Heq, <- Heq'.
@@ -112,31 +113,31 @@ Qed.
 
 Hint Resolve srenvironment_equiv_eq aux_eq aux_diamond : core.
 
-Lemma puts_Empty (n : nat) (R: 𝐄) (V: 𝐕) :
-  (isEmpty(R))%sr -> (isEmpty(puts n R V))%sr.
+Lemma puts_Empty (R: 𝐄)  (V: 𝐕) :
+  (isEmpty(R))%sr -> (isEmpty(puts put R V))%sr.
 Proof.
   intro HEmp; unfold puts.
   rewrite SRE.foldkeys_Empty; auto.
   apply SRE.empty_1.
 Qed.
 
-Lemma puts_Empty_iff (n : nat) (R: 𝐄) (V: 𝐕) :
-  (isEmpty(R))%sr -> ((puts n R V) = ∅)%sr.
+Lemma puts_Empty_iff (R: 𝐄)  (V : 𝐕) :
+  (isEmpty(R))%sr -> ((puts put R V) = ∅)%sr.
 Proof.
   intro HEmp; unfold puts.
   rewrite SRE.foldkeys_Empty; now auto.
 Qed.
 
-Lemma puts_Add (n : nat) (r: resource) (e: Λ) (R R': 𝐄) (V: 𝐕) :
+Lemma puts_Add (r: resource) (e: Λ) (R R': 𝐄) (V: 𝐕) :
   (r ∉ R)%sr -> SRE.Add r e R R' ->
-  (puts n R' V = (⌈r ⤆ put n (r,(put_aux r V))⌉ (puts n R V))%sr)%sr.
+  (puts put R' V = (⌈r ⤆ put (r,(put_aux r V))⌉ (puts put R V))%sr)%sr.
 Proof.
   intros HnIn HAdd.
   unfold puts at 1.
   rewrite SRE.foldkeys_Add; now auto.
 Qed.
 
-#[export] Instance puts_eq (n : nat) : Proper (SRE.eq ==> RE.eq ==> SRE.eq) (puts n).
+#[export] Instance puts_eq : Proper (SRE.eq ==> RE.eq ==> SRE.eq) (puts put).
 Proof.
   intros R R' HeqR V V' HeqV.
   revert R' HeqR.
@@ -145,7 +146,7 @@ Proof.
     -- reflexivity.
     -- now rewrite <- Heq.
   - rewrite puts_Add; eauto.
-    rewrite (puts_Add _ x e R1 R'); auto.
+    rewrite (puts_Add x e R1 R'); auto.
     -- unfold put_aux.
        destruct (V⌊x⌋)%re eqn:Hfi.
        + rewrite HeqV in Hfi.
@@ -158,24 +159,24 @@ Proof.
        now rewrite <- Heq.
 Qed.  
 
-Lemma puts_add (n : nat) (r: resource) (e: Λ) (R: 𝐄) (V: 𝐕) :
+Lemma puts_add (r: resource) (e: Λ) (R: 𝐄) (V: 𝐕) :
   (r ∉ R)%sr ->
-  (puts n (⌈r ⤆ e⌉ R) V = ⌈r ⤆ put n (r,(put_aux r V))⌉ (puts n R V))%sr.
+  (puts put (⌈r ⤆ e⌉ R) V = ⌈r ⤆ put (r,(put_aux r V))⌉ (puts put R V))%sr.
 Proof.
   intro HnIn.
-  rewrite (puts_Add _ r e R); auto.
+  rewrite (puts_Add r e R); auto.
   - reflexivity.
   - apply SRE.Add_add. 
 Qed.
 
-Lemma puts_in_iff (n : nat) (R: 𝐄) (V: 𝐕) (r: resource) :
-  (r ∈ R)%sr <-> (r ∈ (puts n R V))%sr.
+Lemma puts_in_iff (R: 𝐄) (V: 𝐕) (r: resource) :
+  (r ∈ R)%sr <-> (r ∈ (puts put R V))%sr.
 Proof.
   revert r.
   induction R using SRE.map_induction; intro r.
   - split; intros [v HM]; exfalso.
     -- apply (H r v HM).
-    -- apply (puts_Empty n _ V) in H.
+    -- apply (puts_Empty _ V) in H.
        apply (H r v HM).
   - unfold SRE.Add in H0; rewrite H0; clear H0.
     rewrite puts_add; auto.
@@ -183,8 +184,8 @@ Proof.
     now rewrite IHR1.
 Qed.
 
-Lemma puts_new_key (n : nat) (R: 𝐄) (V: 𝐕) :
-  (R⁺)%sr = ((puts n R V)⁺)%sr.
+Lemma puts_new_key (R: 𝐄)  (V: 𝐕) :
+  (R⁺)%sr = ((puts put R V)⁺)%sr.
 Proof.
   induction R using SRE.map_induction.
   - do 2 (rewrite SRE.Ext.new_key_Empty; auto).
@@ -194,25 +195,33 @@ Proof.
     do 2 rewrite SRE.Ext.new_key_add_max; lia.
 Qed.
 
-Lemma puts_Wf (n : nat) (k : lvl) (R : 𝐄) (V : 𝐕) :
-  (forall r v, k ⊩ put n (r,v))%tm ->
-  (k ⊩ R)%sr -> (k ⊩ (puts n R V))%sr.
+Lemma puts_Wf (k : lvl) (R : 𝐄)  (V: 𝐕) :
+  (forall r v, (r ∈ R)%sr -> k ⊩ put (r,v))%tm ->
+  (k ⊩ R)%sr -> (k ⊩ (puts put R V))%sr.
 Proof.
   revert V.
   induction R using SRE.map_induction; intros V Hwfput HwfR.
   - rewrite puts_Empty_iff; auto.
     apply SRE.Wf_empty.
-  - unfold SRE.Add in H0; rewrite H0 in *; clear H0.
+  - unfold SRE.Add in H0; rewrite H0 in *.
     rewrite puts_add; auto.
     apply SRE.Wf_add_notin in HwfR as [Hwfx [_ Hwfe1]]; auto.
     apply SRE.Wf_add_notin.
     -- now rewrite <- puts_in_iff.
     -- repeat (split; auto).
+       + apply Hwfput.
+         rewrite H0.
+         rewrite SRE.add_in_iff; now left.
+       + apply IHR1; auto.
+         intros.
+         apply Hwfput.
+         rewrite H0.
+         rewrite SRE.add_in_iff; now right.
 Qed.
 
-Lemma puts_Wf_V (n : nat) (R : 𝐄) (V : 𝐕) :
-  (forall r v, (V⁺) ⊩ put n (r,v))%tm ->
-  (R⁺)%sr <= V⁺ -> ((V⁺) ⊩ V) -> ((V⁺)%re ⊩ (puts n R V))%sr.
+Lemma puts_Wf_V (R : 𝐄)  (V: 𝐕) :
+  (forall r v, (V⁺) ⊩ put (r,v))%tm ->
+  (R⁺)%sr <= V⁺ -> ((V⁺) ⊩ V) -> ((V⁺)%re ⊩ (puts put R V))%sr.
 Proof.
   revert V.
   induction R using SRE.map_induction; intros V Hwfput Hleq HwfV.
@@ -228,9 +237,9 @@ Proof.
        + apply IHR1; auto; lia. 
 Qed.
 
-Lemma puts_halts (n : nat) (k: lvl) (R : 𝐄) (V : 𝐕) :
-  (forall r v, halts k (put n (r,v)))%tm ->
-  SRE.halts k (puts n R V).
+Lemma puts_halts (k: lvl) (R : 𝐄)  (V: 𝐕) :
+  (forall r v, halts k (put (r,v)))%tm ->
+  SRE.halts k (puts put R V).
 Proof.
   intro Hyput.
   induction R using SRE.map_induction.
@@ -241,9 +250,9 @@ Proof.
     apply SRE.halts_add; split; auto.
 Qed.
 
-Lemma puts_halts_1 (n : nat) (R : 𝐄) (V : 𝐕) :
-  (forall r v, halts (R⁺)%sr (put n (r,v)))%tm ->
-  SRE.halts ((puts n R V)⁺)%sr (puts n R V).
+Lemma puts_halts_1 (R : 𝐄)  (V: 𝐕) :
+  (forall r v, halts (R⁺)%sr (put (r,v)))%tm ->
+  SRE.halts ((puts put R V)⁺)%sr (puts put R V).
 Proof.
   intro Hyput.
   apply puts_halts.
@@ -252,12 +261,12 @@ Proof.
   now apply Hyput.
 Qed.
 
-Lemma puts_find (n : nat) (R : 𝐄) (V : 𝐕) (r: resource) (v: Λ) :
-  (puts n R V ⌊r⌋)%sr = Some v -> exists v', (v = put n (r, v'))%type.
+Lemma puts_find (R : 𝐄) (V: 𝐕) (r: resource) (v: Λ) :
+  (puts put R V ⌊r⌋)%sr = Some v -> exists v', (v = put (r, v'))%type.
 Proof.
   revert r v; induction R using SRE.map_induction; intros r v Hfi. 
   - exfalso.
-    apply (puts_Empty n _ V) in H.
+    apply (puts_Empty _ V) in H.
     apply (H r v).
     now apply SRE.find_2.
   - unfold SRE.Add in H0; rewrite H0 in *; clear H0.
@@ -268,6 +277,8 @@ Proof.
        now exists (put_aux r V).
     -- rewrite SRE.add_neq_o in Hfi; auto.
 Qed.
+
+End put_props.
 
 (** *** [init_input_env] property *)
 
@@ -489,8 +500,8 @@ Qed.
 
 #[export] Instance WF_in_eq : Proper (RContext.eq ==> SRE.eq ==> Logic.eq ==> iff) well_formed_tt.
 Proof.
-  (* intros Rc Rc1 HeqRe R R' HeqS W W' HeqW; subst; split.
-  - intros [HeqDom [HDisj [HvRc [HvS [HvW [Hwt [Hwt' HnEmp ]]]]]]].  
+  intros Rc Rc1 HeqRe R R' HeqS W W' HeqW; subst; split.
+  - intros [HeqDom [HDisj [HvRc [HvS [HvW [Hwt [Hwt' [Hwt'' [HND HnEmp]]]]]]]]].
     split.
     { intro r; rewrite <- HeqS, <- HeqRe; auto. }
     split.
@@ -505,16 +516,21 @@ Proof.
       apply Hwt.
     }
     split.
+    { 
+      intros r r' ty ty' v Hfi HIn.
+      rewrite <- HeqRe in *.
+      eapply Hwt'; eauto.
+    }
+    split.
     {
-      intros r r' v HIn.
-      apply (Hwt' r r' v) in HIn as [α HIn].
-      exists α.
-      now rewrite <- HeqRe.
+      intros r r' ty ty' v Hfi HIn.
+      rewrite <- HeqRe in *.
+      eapply Hwt''; eauto.
     }
     { 
       rewrite <- HeqRe, <- HeqS; auto. 
     }
-  - intros [HeqDom [HDisj [HvRc [HvS [HvW [Hwt [Hwt' HnEmp ]]]]]]].  
+  - intros [HeqDom [HDisj [HvRc [HvS [HvW [Hwt [Hwt' [Hwt'' [HND HnEmp]]]]]]]]].
     split.
     { intro r; rewrite HeqS, HeqRe; auto. }
     split.
@@ -529,17 +545,21 @@ Proof.
       apply Hwt.
     }
     split.
+    { 
+      intros r r' ty ty' v Hfi HIn.
+      rewrite HeqRe in *.
+      eapply Hwt'; eauto.
+    }
+    split.
     {
-      intros r r' v HIn.
-      apply (Hwt' r r' v) in HIn as [α HIn].
-      exists α.
-      now rewrite HeqRe.
+      intros r r' ty ty' v Hfi HIn.
+      rewrite HeqRe in *.
+      eapply Hwt''; eauto.
     }
     { 
       rewrite HeqRe, HeqS; auto. 
     }
-Qed. *)
-Admitted.
+Qed.
 
 Lemma WF_tt_new (Rc : ℜ) (R : 𝐄) (W : 𝐖) :
   WFₜₜ(Rc, R, W) -> (Rc⁺)%rc = max (R⁺)%sr (W⁺)%sk.
@@ -604,19 +624,19 @@ Qed.
 
 (* ---- *)
 
-Lemma temporal_preserves_global_keys (n : nat) (R R': 𝐄) (P P': Λ) (W W' : 𝐖) :
-  # n ⟦R ; W ; P⟧ ⟾ ⟦R' ; W' ; P'⟧ -> (forall (k : resource), (k ∈ R)%sr <-> (k ∈ R')%sr). 
+Lemma temporal_preserves_global_keys (put : resource * (option Λ) -> Λ) (R R': 𝐄) (P P': Λ) (W W' : 𝐖) :
+  # put ⟦R ; W ; P⟧ ⟾ ⟦R' ; W' ; P'⟧ -> (forall (k : resource), (k ∈ R)%sr <-> (k ∈ R')%sr). 
 Proof.
   intros [Vin [Wnew [_tv [_ [Heq _]]]]] k.
   now rewrite Heq; rewrite <- puts_in_iff.
 Qed.
 
-Lemma temporal_preserves_Wf (n : nat) (R R': 𝐄) (P P' : Λ) (W W' : 𝐖) :
-  (forall r v, (R⁺)%sr ⊩ put n (r,v))%tm ->
+Lemma temporal_preserves_Wf (put : resource * (option Λ) -> Λ) (R R': 𝐄) (P P' : Λ) (W W' : 𝐖) :
+  (forall r v, (R⁺)%sr ⊩ put (r,v))%tm ->
   NoDup (ST.keys W) ->
   (~ W = [] -> (W⁺)%sk > (R⁺)%sr) ->
   (R⁺ ⊩ R)%sr -> (W⁺ ⊩ W)%sk -> (max (R⁺)%sr (W⁺)%sk ⊩ P)%tm ->
-  #n ⟦R ; W ; P⟧ ⟾ ⟦R' ; W' ; P'⟧ -> 
+  # put ⟦R ; W ; P⟧ ⟾ ⟦R' ; W' ; P'⟧ -> 
   (R'⁺ ⊩ R')%sr /\ (W'⁺ ⊩ W')%sk /\ (max (R'⁺)%sr (W'⁺)%sk ⊩ P')%tm.
 Proof.
   intros Hwfput HNoD HnEmp HwfS HwfW HwfP [Vout [Wnew [_tv [fT [HeqS HeqW]]]]].
@@ -698,95 +718,393 @@ Qed.
 
 (** ** Preservation - Temporal *)
 
-Hypothesis put_well_behaves : 
-  forall n Rc R, 
-  (forall r, (r ∈ R)%sr -> 
+Definition tT_IO_halts n R W P :=
+  halts n P /\ SRE.halts (R⁺)%sr R /\ ST.halts (W⁺)%sk W.
+
+Lemma tT_inp_to_fT_inp Rc R W P :
+  (Rc ⁺)%rc = Init.Nat.max (R ⁺)%sr (W ⁺)%sk ->
+  (W <> [] -> (W⁺)%sk > (R⁺)%sr) ->
+  tT_IO_halts (Rc⁺)%rc R W P ->
+  fT_inputs_halts (Rc⁺)%rc (init_input_env R W) <[ unit ]> P.
+Proof.
+  intros Heq HnEmp [HltP [HltR HltW]]; split.
+  - unfold init_input_env.
+    rewrite Heq.
+    apply ST.halts_init_locals.
+    -- destruct W eqn:HeqW'.
+       + constructor.
+       + rewrite <- HeqW'.
+         assert (p :: t <> []) by (intro Hc; inversion Hc).
+         apply HnEmp in H.
+         rewrite <- HeqW' in *.
+         now rewrite max_r by lia. 
+    -- apply SRE.halts_init_globals.
+       apply SRE.halts_weakening; auto; lia.
+  - split; auto.
+    exists <[unit]>; split; auto.
+    reflexivity.
+Qed.
+
+Definition tT_outputs_halts n W P :=
+  halts n P /\ ST.halts (W⁺)%sk W.
+
+
+Definition put_good_behavior (put : resource * (option Λ) -> Λ) Rc R := 
+  forall r v, (r ∈ R)%sr -> 
     (forall α β, Rc⌊r⌋%rc = Some (α,β) -> 
-      (forall v,
+      (
         match v with
           | None => True
           | Some v' => ∅%vc ⋅ Rc ⊢ {Term.shift (R⁺)%sr ((Rc⁺)%rc - (R⁺)%sr) v'} ∈ α 
         end ->
-        ((R⁺)%sr ⊩ put n (r,v))%tm /\
-        halts (R⁺)%sr (put n (r,v)) /\
-       ∅%vc ⋅ Rc ⊢ {Term.shift (R⁺)%sr ((Rc⁺)%rc - (R⁺)%sr) (put n (r,v))} ∈ β
+        ∅%vc ⋅ Rc ⊢ {Term.shift (R⁺)%sr ((Rc⁺)%rc - (R⁺)%sr) (put (r,v))} ∈ β
       )
-    )
-  )
+    ) /\
+    ((R⁺)%sr ⊩ put (r,v))%tm /\
+    halts (R⁺)%sr (put (r,v))
 .
 
-Theorem temporal_preserves_typing (n : nat) (Rc : ℜ) (R R': 𝐄) 
+
+
+Theorem temporal_preserves_typing (put : resource * (option Λ) -> Λ)
+                                  (Rc : ℜ) (R R': 𝐄) 
                                   (W W' : 𝐖) (P P' : Λ) (Rs : resources) :
 
-       halts (Rc⁺)%rc P -> SRE.halts (R⁺)%sr R -> ST.halts (W⁺)%sk W ->
-       all_arrow_halting Rc P ->
-                             WFₜₜ(Rc,R,W) -> 
+       tT_IO_halts (Rc⁺)%rc R W P -> halts_arr Rc P ->
+                        WFₜₜ(Rc,R,W) -> 
+                    put_good_behavior put Rc R ->
           
                     ∅%vc ⋅ Rc ⊢ P ∈ (𝟙 ⟿ 𝟙 ∣ Rs) -> 
                       
-                  # n ⟦ R ; W ; P ⟧ ⟾ ⟦ R' ; W' ; P' ⟧ ->
+                  # put ⟦ R ; W ; P ⟧ ⟾ ⟦ R' ; W' ; P' ⟧ ->
   (* ------------------------------------------------------------------------ *)
       exists (Rc1 : ℜ) (Rs' : resources),
             (Rs ⊆ Rs')%s /\ (Rc ⊆ Rc1)%rc /\ WFₜₜ(Rc1,R',W') /\
           
                      ∅%vc ⋅ Rc1 ⊢ P' ∈ (𝟙 ⟿ 𝟙 ∣ Rs') /\ 
      
-      halts (Rc1⁺)%rc P' /\ ST.halts (W'⁺)%sk W' /\ all_arrow_halting Rc1 P'.
+      tT_outputs_halts (Rc1⁺)%rc W' P' /\ halts_arr Rc1 P'.
 Proof.
-  intros HltP HltW HR Harrlt HWF HwtP HTT.
-  assert (HTT': # n ⟦ R; W; P ⟧ ⟾ ⟦ R'; W'; P' ⟧) by assumption.
+  intros Hinplt Harrlt HWF Hpwb HwtP HTT.
+  apply WF_tt_to_WF_ec in HWF as HWF'.
+  apply WF_tt_new in HWF as Hnew.
+  assert (HnEmp: W <> [] -> (W ⁺)%sk > (R ⁺)%sr).
+  {
+    destruct HWF as [_ [_ [_ [_ [_ [_ [_ [_ [_ ]]]]]]]]].
+    intro HI; apply H in HI as []; assumption.
+  }
+  apply tT_inp_to_fT_inp in Hinplt as Hinplt'; auto.
+  assert (HTT': # put ⟦ R; W; P ⟧ ⟾ ⟦ R'; W'; P' ⟧) by assumption.
   destruct HTT as [Vout [Wnew [_tv [HfT [HeqR HeqW]]]]].
+  apply functional_W_props in HfT as HI.
+  destruct HI as [HND [HeqDom HnEmp']].
 
-  apply Functional_Transition.functional_preserves_typing_gen 
-  with (Rc := Rc) (α := <[𝟙]>) (β := <[𝟙]>) (R := Rs)
-  in HfT; auto.
-  - destruct HfT as [Hunsd [Hunsd' [Rc1 [Rs' [HsubRc [HsubRs 
-                    [Hout [Harrlt' [Hwt [Hwt' [HWF' [HwW [Hdisj Husd]]]]]]]]]]]]]. 
+  apply functional_preserves_keys in HfT as HI.
+  destruct HI as [HIn Hle].
+
+  apply functional_preserves_Wf in HfT as HI; auto.
+  - destruct HI as [HwfVout [_ [HwfP' [HwfWnew HleVout]]]].
+
+    apply Functional_Transition.functional_preserves_typing 
+    with (Rc := Rc) (α := <[𝟙]>) (β := <[𝟙]>) (R := Rs)
+    in HfT; auto.
+    destruct HfT as [Hunsd [Hunsd' [Rc1 [Rs' [HsubRc [HsubRs 
+                      [Hout [Harrlt' [Hwt [Hwt' [HWF'' [HwW [Hdisj Husd]]]]]]]]]]]]]. 
     exists Rc1, Rs'.
     do 3 (split; auto).
-    {
-      destruct HWF 
-      as [HeqDom [Hdisj' [HwfRc [HwfR [HwfW [HwtR [HwtW [HnDup HnewW]]]]]]]].
-      destruct HWF' as [HeqDom' [HwfRc1 [HwfVout HwtV]]].
-      split.
+    { 
+      split. 
+      {
+        intro r. 
+        rewrite HeqR, HeqW.
+        rewrite ST.update_locals_keys_In.
+        rewrite <- puts_in_iff.
+        rewrite ST.keys_in_app.
+        rewrite ST.keys_in_shift_new_key.
+        clear HTT' HwW Hunsd Hunsd' Hpwb.
+        rewrite (WF_ec_In Rc1 Vout); auto.
+        split.
+        - intro HInVout.
+          specialize (HeqDom r).
+          rewrite RE.diff_in_iff in HeqDom.
+          rewrite <- init_input_env_in_iff in HeqDom.
+          destruct (List.In_dec Resource.eq_dec r (ST.keys W)) as [|HnInW]; auto.
+          destruct (SRE.In_dec R r) as [|HnInR]; auto.
+          left; right.
+          rewrite <- HeqDom; split; auto.
+          now intros [|].
+        - intros [[HInW|HInWnew]|HInR].
+          -- apply HIn.
+             rewrite <- init_input_env_in_iff; auto.
+          -- rewrite <- HeqDom in HInWnew.
+             rewrite RE.diff_in_iff in HInWnew.
+             now destruct HInWnew.
+          -- apply HIn.
+             rewrite <- init_input_env_in_iff; auto.
+      } 
+      split. 
+      {
+        intros r.
+        rewrite HeqW, HeqR.
+        rewrite ST.update_locals_keys_In.
+        rewrite <- puts_in_iff.
+        rewrite ST.keys_in_app.
+        rewrite ST.keys_in_shift_new_key.
+        clear HTT' HwW Hunsd Hunsd' Hpwb.
+        intros [HInW | HInWnew].
+        - destruct HWF as [_ []]; auto.
+        - rewrite <- HeqDom in HInWnew.
+          rewrite RE.diff_in_iff in HInWnew.
+          destruct HInWnew as [_ HIninp].
+          rewrite <- init_input_env_in_iff in HIninp.
+          intro c; apply HIninp; auto.
+      } 
+      split. 
+      { now apply WF_ec_Wf in HWF'' as []. } 
+      split. 
+      {
+        rewrite HeqR.
+        rewrite <- puts_new_key.
+        apply puts_Wf.
+        - intros. destruct (Hpwb r v); auto.
+          now destruct H1.
+        - now destruct HWF as [_ [_ [_ []]]]. 
+      } 
+      split. 
+      {
+        clear Hpwb Hwt Hwt' Harrlt' HTT' HeqR Hunsd Hunsd' HwW Husd.
+        destruct W, Wnew.
+        - simpl in *.
+          rewrite HeqW.
+          apply ST.Wf_nil.
+        - remember (p :: Wnew) as Wnew'; clear HnEmp.
+          simpl in *.
+          rewrite HeqW.
+          destruct HnEmp'.
+          -- subst; intro c; inversion c.
+          -- rewrite ST.update_locals_new_key.
+             apply ST.update_locals_Wf; split; rewrite <- H; auto.
+        - remember (p :: W) as W1; clear HnEmp'.
+          simpl in *.
+          rewrite HeqW.
+          rewrite app_nil_r in *.
+          assert (W1 <> []) by (subst; intro c; inversion c).
+          apply HnEmp in H.
+          assert (Vout⁺ <= (init_input_env R W1)⁺).
+          { 
+            apply RE.new_key_incl.
+            now apply RE.diff_in_false.
+          }
+          rewrite init_input_env_new_key in *.
+          rewrite max_r in * by lia.
+          assert (Vout⁺ = W1⁺%sk) by lia.
+          rewrite H1.
+          rewrite ST.update_locals_new_key.
+          replace (W1 ⁺ - W1 ⁺)%sk with 0 by lia.
+          rewrite ST.shift_zero_refl.
+          destruct HWF as [_ [_ [_ [_ []]]]].
+          apply ST.update_locals_Wf; split; auto; rewrite <- H1; auto.
+        - remember (p :: W) as W1.
+          remember (p0 :: Wnew) as Wnew1.
+          destruct HnEmp'.
+          { subst; intro c; inversion c. }
+          assert (W1 <> []) by (subst; intro c; inversion c).
+          apply HnEmp in H1; clear HnEmp.
+          rewrite init_input_env_new_key in *.
+          rewrite max_r in * by lia.
+          rewrite HeqW.
+          rewrite ST.update_locals_new_key.
+          rewrite ST.new_key_app.
+          rewrite ST.new_key_shift_refl; auto.
+          rewrite max_r by lia.
+          rewrite <- H.
+          apply ST.update_locals_Wf; split; auto.
+          apply ST.Wf_app; split; auto.
+          apply ST.shift_preserves_wf_2; auto.
+          destruct HWF as [_ [_ [_ [_ [ ]]]]]; assumption.
+      } 
+      split. 
       { 
-        intro r.
-        rewrite <- temporal_preserves_global_keys; eauto.
-        rewrite HeqW.
-        admit.
+        intros r [ty ty'] v HfiRc1.
+        rewrite HeqR, HeqW.
+        rewrite <- puts_new_key.
+        rewrite ST.update_locals_new_key.
+        rewrite ST.new_key_app.
+        rewrite ST.new_key_shift_refl; auto.
+        unfold put_good_behavior in Hpwb.
+        simpl in *.
+        intro HfiR.
+        assert (HInR : (r ∈ R)%sr).
+        { 
+          rewrite puts_in_iff.
+          exists v.
+          apply SRE.find_2 in HfiR; eauto. 
+        }
+        specialize (Hpwb r (Some v) HInR).
+        destruct Hpwb as [Hwtput _].
+        apply puts_find in HfiR as HI.
+        destruct HI as [v' Heq]; subst.
+        admit. 
+      } 
+      split. 
+      {
+        intros r r' ty ty' v Hfi HInW'.
+        rewrite HeqW in HInW'.
+        apply ST.update_locals_In in HInW' as [[HInW' Hnfi]|[v'[HInW' HfiVout]]].
+        - apply List.in_app_or in HInW' as [HInW|HInWnew].
+          -- admit.
+          -- apply HwW in HInWnew as [τ [Hwtv [HfiRc1 HfiRc1']]].
+             rewrite Hfi in HfiRc1.
+             inversion HfiRc1; subst; split; auto.
+        - apply List.in_app_or in HInW' as [HInW|HInWnew].
+          -- admit.
+          -- apply HwW in HInWnew as [τ [Hwtv [HfiRc1 HfiRc1']]].
+             rewrite Hfi in HfiRc1.
+             inversion HfiRc1; subst; split; auto.
+             destruct HWF'' as [_ [_ [_ H]]].
+             apply H with (v := (Cell.out v)) in HfiRc1'; auto.
+      } 
+      split. 
+      { 
+        intros r r' ty ty' v Hfi HInW'.
+        rewrite HeqW in HInW'.
+        apply ST.update_locals_In in HInW' as [[HInW' Hnfi]|[v'[HInW' HfiVout]]].
+        - apply List.in_app_or in HInW' as [HInW|HInWnew].
+          -- admit.
+          -- apply HwW in HInWnew as [τ [Hwtv [HfiRc1 HfiRc1']]].
+             rewrite Hfi in HfiRc1'.
+             inversion HfiRc1'; subst; split; auto.
+        - apply List.in_app_or in HInW' as [HInW|HInWnew].
+          -- admit.
+          -- apply HwW in HInWnew as [τ [Hwtv [HfiRc1 HfiRc1']]].
+             rewrite Hfi in HfiRc1'.
+             inversion HfiRc1'; subst; split; auto.
+             destruct HWF'' as [_ [_ [_ H]]].
+             apply H with (v := (Cell.out v)) in Hfi; auto.
       }
       split.
-      { admit. }
-      split; auto.  
-    admit. }
-    do 2 (split; auto).
-    { now destruct Hout as [_ [_ [_ ]]]. }
-    split; auto.
-    { 
-      rewrite HeqW.
-      rewrite ST.update_locals_new_key.
-      rewrite ST.new_key_app.
-      rewrite ST.new_key_shift_refl; auto.
-      apply ST.halts_update_locals;
-      admit. 
+      { 
+        rewrite HeqW.
+        apply ST.update_locals_NoDup_keys.
+        apply ST.NoDup_keys_app; auto.
+        - apply ST.NoDup_keys_shift.
+          now destruct HWF as [_ [_ [_ [_ [_ [_ [_ [_ [ ]]]]]]]]].
+        - intro r.
+          rewrite <- HeqDom.
+          rewrite RE.diff_in_iff; intros [HInVout HIninp].
+          rewrite <- init_input_env_in_iff in HIninp.
+          rewrite ST.keys_in_shift_new_key.
+          intro c; apply HIninp; auto.
+      }
+      { 
+        rewrite HeqW, HeqR.
+        rewrite <- puts_new_key.
+        rewrite ST.update_locals_new_key.
+        rewrite ST.new_key_app.
+        rewrite ST.new_key_shift_refl; auto.
+        intro Hnnil.
+        rewrite ST.update_locals_not_nil in Hnnil.
+        apply ST.app_not_nil in Hnnil.
+        rewrite ST.shift_not_nil in Hnnil.
+        destruct Hnnil as [Hnnil|Hnnil].
+        - apply HnEmp in Hnnil.
+          split; try lia. 
+          destruct Wnew.
+          -- simpl in *.
+             rewrite max_l by lia.
+             assert (Vout⁺ <= (init_input_env R W)⁺).
+             { 
+              apply RE.new_key_incl.
+              now apply RE.diff_in_false. 
+             }
+             assert (Vout⁺ = (init_input_env R W)⁺) by lia.
+             rewrite (WF_ec_new Rc1 Vout); auto.
+             rewrite H0.
+             rewrite init_input_env_new_key; lia.
+          -- remember (p :: Wnew) as Wnew'.
+             destruct HnEmp'.
+             + subst; intro c; inversion c.
+             + rewrite init_input_env_new_key in H0.
+               rewrite max_r by lia.
+               rewrite (WF_ec_new Rc1 Vout); auto.
+        - apply HnEmp' in Hnnil as [Heq Hle']; rewrite <- Heq in *.
+          rewrite init_input_env_new_key in Hle'.
+          rewrite (WF_ec_new Rc1 Vout); auto.
+          split; lia.
+      } 
     }
-  - repeat split; auto.
-    -- unfold init_input_env.
-       apply WF_tt_new in HWF as Hnew.
-       rewrite Hnew.
-       apply ST.halts_init_locals; auto.
-       + destruct W eqn:HeqW'.
-         ++ constructor.
-         ++ rewrite <- HeqW'.
-            destruct HWF as [_ [_ [_ [_ [_ [_ [_ [_ [_ ]]]]]]]]].
-            destruct H.
-            * intro Hc; inversion Hc.
-            * rewrite <- HeqW' in *.
-              now rewrite max_r by lia.
-       + apply SRE.halts_init_globals.
-         apply SRE.halts_weakening; auto; lia.
-    -- exists <[unit]>; split; auto; reflexivity.
-  - now apply WF_tt_to_WF_ec.
+    do 2 (split; auto).
+    { 
+      clear Hpwb Hwt Hwt' Harrlt' HTT' HeqR Hunsd Hunsd' HwW Husd.
+      split; auto.
+      - destruct Hout as [_ [_ []]]; auto.
+      - destruct W, Wnew.
+        -- simpl in *; rewrite HeqW.
+          apply ST.halts_nil.
+        -- remember (p :: Wnew) as Wnew'.
+          rewrite HeqW in *; simpl in *.
+          destruct HnEmp'.
+          + rewrite HeqWnew'; intro Hc; inversion Hc.
+          + rewrite ST.update_locals_new_key.
+            rewrite <- H.
+            rewrite <- (WF_ec_new Rc1 Vout); auto.
+            destruct Hout as [HoutV [HoutW ]].
+            now apply ST.halts_update_locals.
+        -- remember (p :: W) as W1.
+          clear HnEmp'.
+          rewrite HeqW in *; simpl in *.
+          rewrite app_nil_r in *.
+          assert (Vout⁺ <= (init_input_env R W1)⁺).
+          { 
+            apply RE.new_key_incl.
+            now apply RE.diff_in_false.
+          }
+          assert (W1 <> []) by (subst; intro c; inversion c).
+          apply HnEmp in H0.
+          rewrite init_input_env_new_key in *.
+          rewrite max_r in * by lia.
+          replace ((Vout⁺)%re - W1⁺)%sk with 0 by lia.
+          rewrite ST.update_locals_new_key.
+          rewrite ST.shift_zero_refl.
+          destruct Hout as [HoutV _].
+          destruct Hinplt as [_ [HltR HltW1]].
+          apply ST.halts_update_locals; auto.
+          assert ((W1⁺)%sk = Vout⁺) by lia.
+          rewrite H1.
+          rewrite <- (WF_ec_new Rc1 Vout); auto.
+        -- remember (p0 :: Wnew) as Wnew'.
+          remember (p :: W) as W1.
+          assert (W1 <> []).
+          { subst; intro c; inversion c. }
+          apply HnEmp in H; clear HnEmp.
+          rewrite init_input_env_new_key in *.
+          rewrite max_r in * by lia.
+          assert (Wnew' <> []).
+          { subst; intro c; inversion c. }
+          apply HnEmp' in H0; clear HnEmp'.
+          destruct H0 as [Heq Hlt].
+          rewrite HeqW.
+          rewrite ST.update_locals_new_key.
+          rewrite ST.new_key_app.
+          rewrite ST.new_key_shift_refl; auto.
+          rewrite max_r by lia.
+          destruct Hout as [HoutV [HoutW]].
+          destruct Hinplt as [_ [HltR HltW1]].
+          apply ST.halts_update_locals; auto.
+          + rewrite <- Heq.
+            rewrite <- (WF_ec_new Rc1 Vout); auto.
+          + apply ST.halts_app; split.
+            ++ rewrite Heq.
+                apply ST.halts_weakening; auto; lia.
+            ++ rewrite <- Heq.
+                rewrite <- (WF_ec_new Rc1 Vout); auto.
+    }
+  - destruct HWF as [_ [_ [HwfRc [HwfR []]]]]. 
+    apply init_input_env_Wf; auto.
+  - constructor.
+  - rewrite <- (WF_ec_new Rc); auto.
+    apply well_typed_implies_Wf in HwtP as []; auto.
+    now destruct HWF as [_ [_ []]].
 Admitted.
 
 (** ---- *)
@@ -794,7 +1112,7 @@ Admitted.
 
 (** ** Progress - Temporal *)
 
-(* Theorem temporal_progress (n : nat) (Rc : ℜ) (R : resources) (W: 𝐖) (P : Λ) (Rs : resources) :
+(* Theorem temporal_reactivity (n : nat) (Rc : ℜ) (R : resources) (W: 𝐖) (P : Λ) (Rs : resources) :
 
           halts (Rc⁺)%rc P -> ST.halts (W⁺)%sk W ->
  
@@ -806,6 +1124,3 @@ Admitted.
 Proof. admit.
 
 Admitted. *)
-
-
-End temporal.
